Move some deprecated code into MemoryExplore

common/MemoryExplore.v
@@ -15,8 +15,398 @@ Require Import Lia.
 Require Import MemoryC.
 
 Require Import Events.
-Import Mem.
 Local Notation "a # b" := (PMap.get b a) (at level 1).
+
+
+
+
+
+
+
+
+
+
+
+
+
+
+
+
+
+
+Program Definition Mem_drop_perm_none (m: mem) (b: block) (lo hi: Z): mem :=
+  (Mem.mkmem m.(Mem.mem_contents)
+                 (PMap.set b
+                           (fun ofs k =>
+                              if zle lo ofs && zlt ofs hi
+                              then None
+                              else m.(Mem.mem_access)#b ofs k)
+                           m.(Mem.mem_access))
+                 m.(Mem.nextblock) _ _ _)
+.
+Next Obligation.
+  repeat rewrite PMap.gsspec.
+  destruct (peq b0 b); cycle 1.
+  { apply Mem.access_max. }
+  subst.
+  des_ifs.
+  - apply Mem.access_max.
+Qed.
+Next Obligation.
+  hexploit Mem.nextblock_noaccess; eauto; []; i; des.
+  rewrite PMap.gsspec.
+  des_ifs; eauto.
+Qed.
+Next Obligation.
+  apply Mem.contents_default.
+Qed.
+
+Lemma Mem_drop_perm_none_spec
+      m0 blk0 lo hi m1
+      (DROP: Mem_drop_perm_none m0 blk0 lo hi = m1)
+  :
+    (<<NB: Mem.nextblock m0 = Mem.nextblock m1>>)
+    /\
+    (<<UNCH: Mem.unchanged_on (fun blk1 ofs => blk0 <> blk1 \/ ofs < lo \/ hi <= ofs) m0 m1>>)
+    /\
+    (<<INSIDE: forall
+        ofs
+        (INSIDE: lo <= ofs < hi)
+    ,
+      all2 ~2 Mem.perm m1 blk0 ofs>>)
+.
+Proof.
+  ii.
+  unfold Mem_drop_perm_none in *. des_ifs.
+  unfold Mem.perm in *. ss. rewrite PMap.gsspec in *. des_ifs.
+  splits; ii; ss.
+  - econs; ss; eauto.
+    { reflexivity. }
+    ii.
+    unfold Mem.perm. cbn. rewrite ! PMap.gsspec in *. des_ifs. simpl_bool.
+    des; ss; des_sumbool; try lia.
+  - des_ifs. simpl_bool. des; des_sumbool; lia.
+Qed.
+
+Lemma Mem_set_perm_none_impl
+      m0 blk lo hi m1
+      (DROP: Mem_drop_perm_none m0 blk lo hi = m1)
+  :
+    <<PERM: Mem.perm m1 <4= Mem.perm m0>>
+.
+Proof.
+  ii.
+  unfold Mem_drop_perm_none in *. des_ifs.
+  unfold Mem.perm in *. ss. rewrite PMap.gsspec in *. des_ifs.
+Qed.
+
+Lemma Mem_set_perm_none_left_inject
+      `{Val.meminj_ctx}
+      j m_src0 m_tgt0
+      (INJ: Mem.inject j m_src0 m_tgt0)
+      blk lo hi m_src1
+      (DROP: Mem_drop_perm_none m_src0 blk lo hi = m_src1)
+  :
+    <<INJ: Mem.inject j m_src1 m_tgt0>>
+.
+Proof.
+  hexploit Mem_set_perm_none_impl; eauto. intro IMPL; des.
+  inv INJ.
+  unfold Mem_drop_perm_none in *. des_ifs.
+  unfold Mem.perm in IMPL. ss.
+  econs; ss; eauto.
+  - inv mi_inj.
+    econs; i; ss; eauto.
+    + exploit mi_perm; eauto.
+      eapply IMPL; eauto.
+    + eapply mi_align; eauto.
+      ii.
+      eapply IMPL; eauto. eapply H1; eauto.
+    + exploit mi_memval; eauto.
+      eapply IMPL; eauto.
+  - ii. unfold Mem.perm in *. ss. eapply mi_no_overlap; eauto; eapply IMPL; eauto.
+  - unfold Mem.perm. ss.
+    ii. eapply mi_representable; eauto.
+    des.
+    + left. eapply IMPL; eauto.
+    + right. eapply IMPL; eauto.
+  - ii. hexploit mi_perm_inv; eauto.
+    unfold Mem.perm. ss. unfold Mem.perm in H1.
+    i; des.
+    + rewrite PMap.gsspec in *. des_ifs; ss; eauto.
+    + rewrite PMap.gsspec in *. des_ifs; ss; eauto.
+Qed.
+
+Global Opaque Mem_drop_perm_none.
+
+
+
+
+
+
+
+
+Module DEPRECATED.
+
+Program Definition Mem_set_perm (m: mem) (b: block) (lo hi: Z) (op: option permission): option mem :=
+  match op with
+    | Some p =>
+      if (Mem.range_perm_dec m b lo hi Max p) then
+        if (plt b m.(Mem.nextblock)) then
+          Some (Mem.mkmem m.(Mem.mem_contents)
+                          (PMap.set b
+                                    (fun ofs k =>
+                                       match k with
+                                         | Cur =>
+                                           if zle lo ofs && zlt ofs hi
+                                           then Some p
+                                           else m.(Mem.mem_access)#b ofs k
+                                         | Max => m.(Mem.mem_access)#b ofs k
+                                       end
+                                    )
+                                    m.(Mem.mem_access))
+                          m.(Mem.nextblock) _ _ _)
+        else None
+      else None
+    | None =>
+      Some (Mem.mkmem m.(Mem.mem_contents)
+                      (PMap.set b
+                                (fun ofs k =>
+                                   if zle lo ofs && zlt ofs hi
+                                   then None
+                                   else m.(Mem.mem_access)#b ofs k)
+                                m.(Mem.mem_access))
+                      m.(Mem.nextblock) _ _ _)
+  end.
+Next Obligation.
+  repeat rewrite PMap.gsspec.
+  destruct (peq b0 b); cycle 1.
+  { apply Mem.access_max. }
+  subst.
+  des_ifs.
+  - simpl_bool; des; des_sumbool.
+    exploit H; eauto.
+  - apply Mem.access_max.
+Qed.
+Next Obligation.
+  specialize (Mem.nextblock_noaccess m b0 ofs k H1). intros.
+  rewrite PMap.gsspec.
+  des_ifs.
+Qed.
+Next Obligation.
+  apply Mem.contents_default.
+Qed.
+Next Obligation.
+  repeat rewrite PMap.gsspec. destruct (peq b0 b). subst b0.
+  destruct (zle lo ofs && zlt ofs hi). red; auto with mem. apply Mem.access_max.
+  apply Mem.access_max.
+Qed.
+Next Obligation.
+  hexploit Mem.nextblock_noaccess; eauto; []; i; des.
+  rewrite PMap.gsspec.
+  des_ifs; eauto.
+Qed.
+Next Obligation.
+  apply Mem.contents_default.
+Qed.
+
+Lemma Mem_set_perm_none_spec
+      m0 blk0 lo hi m1
+      (DROP: Mem_set_perm m0 blk0 lo hi None = Some m1)
+  :
+    (<<OUTSIDE: forall
+      blk1 ofs
+      (DISJOINT: blk0 <> blk1 \/ ofs < lo \/ hi <= ofs)
+    ,
+      all2 (Mem.perm m0 blk1 ofs <2> Mem.perm m1 blk1 ofs)>>)
+    /\
+    (<<INSIDE: forall
+        ofs
+        (INSIDE: lo <= ofs < hi)
+    ,
+      all2 ~2 Mem.perm m1 blk0 ofs>>)
+.
+Proof.
+  ii.
+  unfold Mem_set_perm in *. des_ifs.
+  unfold Mem.perm in *. ss. rewrite PMap.gsspec in *. des_ifs.
+  split; ii; ss.
+  - rewrite PMap.gsspec.
+    des_ifs. simpl_bool. des_safe. des_sumbool. admit "IDK WHY BUT IT MAKES xomega SLOW IN STACKINGPROOFC1.v!!!!!! des; try xomega".
+  - des_ifs. simpl_bool. des_safe. admit "des; des_sumbool; try xomega".
+Qed.
+
+Lemma Mem_set_perm_none_impl
+      m0 blk lo hi m1
+      (DROP: Mem_set_perm m0 blk lo hi None = Some m1)
+  :
+    <<PERM: Mem.perm m1 <4= Mem.perm m0>>
+.
+Proof.
+  ii.
+  unfold Mem_set_perm in *. des_ifs.
+  unfold Mem.perm in *. ss. rewrite PMap.gsspec in *. des_ifs.
+Qed.
+
+Lemma Mem_set_perm_none_left_inject
+      `{Val.meminj_ctx}
+      j m_src0 m_tgt0
+      (INJ: Mem.inject j m_src0 m_tgt0)
+      blk lo hi m_src1
+      (DROP: Mem_set_perm m_src0 blk lo hi None = Some m_src1)
+  :
+    <<INJ: Mem.inject j m_src1 m_tgt0>>
+.
+Proof.
+  hexploit Mem_set_perm_none_impl; eauto. intro IMPL; des.
+  inv INJ.
+  unfold Mem_set_perm in *. des_ifs.
+  unfold Mem.perm in IMPL. ss.
+  econs; ss; eauto.
+  - inv mi_inj.
+    econs; i; ss; eauto.
+    + exploit mi_perm; eauto.
+      eapply IMPL; eauto.
+    + eapply mi_align; eauto.
+      ii.
+      eapply IMPL; eauto. eapply H1; eauto.
+    + exploit mi_memval; eauto.
+      eapply IMPL; eauto.
+  - ii. unfold Mem.perm in *. ss. eapply mi_no_overlap; eauto; eapply IMPL; eauto.
+  - unfold Mem.perm. ss.
+    ii. eapply mi_representable; eauto.
+    des.
+    + left. eapply IMPL; eauto.
+    + right. eapply IMPL; eauto.
+  - ii. hexploit mi_perm_inv; eauto.
+    unfold Mem.perm. ss. unfold Mem.perm in H1.
+    i; des.
+    + rewrite PMap.gsspec in *. des_ifs; ss; eauto.
+    + rewrite PMap.gsspec in *. des_ifs; ss; eauto.
+Qed.
+
+Global Opaque Mem_set_perm.
+
+(* heap(malloc) has permission on (b, -1) *)
+(* TODO: Name is not precise... malloc && drop_perm will satsify this condition. *)
+Definition is_stack_block (m: mem) (blk: block): Prop := forall
+    ofs kind perm
+    (PERM: Mem.perm m blk ofs kind perm)
+  ,
+    <<POS: 0 <= ofs>>
+.
+Hint Unfold is_stack_block.
+
+End DEPRECATED.
+
+Definition dead_block (m: mem) (b: block): Prop := forall ofs, ~Mem.perm m b ofs Cur Nonempty.
+
+Inductive mem_equiv (m0 m1: mem): Prop :=
+| mem_equiv_intro
+    (UNCH: Mem.unchanged_on top2 m0 m1)
+    (DEAD: forall b (BETWEEN: (m0.(Mem.nextblock) <= b < m1.(Mem.nextblock))%positive), dead_block m1 b)
+.
+
+Lemma Mem_unchanged_on_trans_strong
+      P m0 m1 m2
+      (UNCH0: Mem.unchanged_on P m0 m1)
+      (UNCH1: Mem.unchanged_on (P /2\ (fun b _ => Mem.valid_block m0 b)) m1 m2)
+  :
+    <<UNCH2: Mem.unchanged_on P m0 m2>>
+.
+Proof.
+  inv UNCH0. inv UNCH1.
+  econs; i.
+  - xomega.
+  - etransitivity.
+    { eapply unchanged_on_perm; eauto. }
+    eapply unchanged_on_perm0; eauto.
+    { unfold Mem.valid_block in *. xomega. }
+  - erewrite <- unchanged_on_contents; eauto.
+    dup H0. apply Mem.perm_valid_block in H1. unfold Mem.valid_block in *.
+    erewrite <- unchanged_on_contents0; eauto.
+    eapply unchanged_on_perm; eauto.
+Qed.
+
+Lemma drop_perm_none_dead_block
+      m0 blk lo hi
+      (INSIDE: forall ofs k p (PERM: Mem.perm m0 blk ofs k p), lo <= ofs < hi)
+  :
+    dead_block (Mem_drop_perm_none m0 blk lo hi) blk
+.
+Proof.
+  ii.
+  exploit (Mem_drop_perm_none_spec m0 blk lo hi); eauto. i; des.
+  destruct (classic (lo <= ofs < hi)).
+  - eapply INSIDE0; eauto.
+  - inv UNCH.
+    erewrite <- unchanged_on_perm in *; ss.
+    + eapply INSIDE in H. xomega.
+    + right. xomega.
+    + unfold Mem.valid_block. rewrite NB.
+      eapply Mem.perm_valid_block; eauto.
+Qed.
+
+Lemma Mem_alloc_range_perm
+      m0 lo hi m1 blk
+      (ALLOC: Mem.alloc m0 lo hi = (m1, blk))
+  :
+    <<PERM: Mem.range_perm m1 blk lo hi Cur Freeable>>
+.
+Proof.
+  ii. eapply Mem.perm_alloc_2; eauto.
+Qed.
+
+Hint Resolve Mem_alloc_range_perm : mem.
+
+
+
+Inductive future_imm (m0 m1: mem): Prop :=
+| future_imm_alloc
+    blk lo hi
+    (FREE: Mem.alloc m0 lo hi = (m1, blk))
+| future_imm_store
+    chunk blk ofs v
+    (STORE: Mem.store chunk m0 blk ofs v = Some m1)
+| future_imm_storebytes
+    ofs blk mvs
+    (STOREB: Mem.storebytes m0 blk ofs mvs = Some m1)
+| future_imm_free
+    blk lo hi
+    (FREE: Mem.free m0 blk lo hi = Some m1)
+| future_imm_drop_perm_none
+    blk lo hi
+    (DROPN: Mem_drop_perm_none m0 blk lo hi = m1)
+(* TODO: drop_perm? *)
+.
+Hint Constructors future_imm.
+
+Definition future: mem -> mem -> Prop := rtc future_imm.
+Hint Unfold future.
+
+
+
+
+
+
+
+
+
+
+
+
+
+
+
+
+
+
+
+
+
+
+
+Import Mem.
 
 Local Existing Instance Val.mi_normal.
 
